rocq-skylabs-brick/theories/lang/cpp/syntax/pretty.v
@@ -83,9 +83,9 @@ Section with_lang.
                 end in
       concat $ join_sep " " $ (c ++ v ++ vc)%list.
 
-    Fixpoint printAN (an : atomic_name) : PrimString.string :=
+    Definition printAN (an : atomic_name) : PrimString.string :=
       let print_args args := parens $ concat $ join_sep ", " $ printType <$> args in
-      match an with
+      match drop_atomic_name_loc_info an with
       | Nid id => id
       | Nfunction quals nm args =>
           nm ++ print_args args ++ with_space (printFQ quals)
@@ -108,7 +108,7 @@ Section with_lang.
       | Nfirst_decl n => "#" ++ n
       | Nfirst_child n => "." ++ n
       | Nunsupported_atomic note => "?" ++ note
-      | ANLocInfo _ an => printAN an
+      | ANLocInfo _ _ => "<location>" (* unreachable *)
       end.
   End atomic_name.
 
